Incremental/LawfulEST.lean
@@ -1,0 +1,40 @@
+module
+
+public import Init.Control.Lawful.MonadAttach.Lemmas
+public import Init.System.ST
+public import Init.System.IO
+
+@[expose] public section
+
+namespace Incremental
+
+variable {ε σ : Type}
+
+/-!
+We use `EST` but we can't actually prove anything about it.
+Just assume it's well behaved.
+
+If you define a build system that, for example, checks a boolean "cancelled?" flag in another thread,
+you need `IO`. Same thing if you need to benchmark queries, with `IO.monoNanosNow` for example.
+We aren't relying on these for soundness anyway, if you really want verifiability, just don't use those build systems.
+-/
+
+axiom EST.instLawfulMonad : LawfulMonad (EST ε σ)
+attribute [instance] EST.instLawfulMonad
+
+axiom EST.lawfulMonadAttach : LawfulMonadAttach (EST ε σ)
+attribute [instance] EST.lawfulMonadAttach
+
+instance : LawfulMonad (EIO ε) := inferInstanceAs (LawfulMonad (EST ε IO.RealWorld))
+instance : LawfulMonadAttach (EIO ε) := inferInstanceAs (LawfulMonadAttach (EST ε IO.RealWorld))
+
+axiom ST.instLawfulMonad : LawfulMonad (ST σ)
+attribute [instance] ST.instLawfulMonad
+
+axiom ST.lawfulMonadAttach : LawfulMonadAttach (ST σ)
+attribute [instance] ST.lawfulMonadAttach
+
+instance : LawfulMonad BaseIO := inferInstanceAs (LawfulMonad (ST IO.RealWorld))
+instance : LawfulMonadAttach BaseIO := inferInstanceAs (LawfulMonadAttach (ST IO.RealWorld))
+
+end Incremental
