Incremental/Shake/C.lean
@@ -1,6 +1,6 @@
 module
 
-public import Incremental.ShakeStore
+public import Incremental.Shake.Store
 
 namespace Incremental
 
@@ -12,12 +12,7 @@ variable
   [BEq ℭ.I] [LawfulBEq ℭ.I] [Hashable ℭ.I] [∀ i, Hashable (ℭ.V i)]
   [BEq ℭ.Q] [LawfulBEq ℭ.Q] [Hashable ℭ.Q] [∀ q, Hashable (ℭ.R q)]
 
-instance
-    {ℭ : BuildConfig}
-    [BEq ℭ.I] [Hashable ℭ.I] [∀ i, Hashable (ℭ.V i)]
-    [BEq ℭ.Q] [Hashable ℭ.Q] [∀ q, Hashable (ℭ.R q)]
-    {J : Type} [Input ℭ J] :
-    Inhabited (Tasks Monad ℭ → ∀ q, ShakeRT.Store ℭ J → ℭ.R q × ShakeRT.Store ℭ J) :=
+instance : Inhabited (Tasks Monad ℭ → ∀ q, ShakeRT.Store ℭ J → ℭ.R q × ShakeRT.Store ℭ J) :=
   ⟨sorry⟩
 
 @[extern "lean_shake_build"]
@@ -29,7 +24,7 @@ public opaque shakeCBuild
     Tasks Monad ℭ → ∀ q,
     ShakeRT.Store ℭ J → ℭ.R q × ShakeRT.Store ℭ J
 
-@[expose] public def ShakeC (tasks : Tasks Monad ℭ) : Build Monad ℭ J tasks Id where
+@[expose] public def ShakeC (tasks : Tasks Monad ℭ) : Build Monad ℭ J tasks Id Id where
   cId := Id.instMonad
   σ := ShakeRT.Store ℭ J
   init inputs := {
