Incremental/Test/Fibonacci.lean
@@ -1,0 +1,29 @@
+import Incremental.Basic
+
+namespace Incremental.Test.Fibonacci
+
+abbrev config : Incremental.BuildConfig where
+  I := Empty
+  V := nofun
+  Q := Nat
+  R _ := Nat
+  rel := (· < ·)
+  wf := Nat.lt_wfRel.wf
+
+instance : Incremental.Input config Unit where
+  get := nofun
+  set := nofun
+  get_set_self := nofun
+  get_set_other := nofun
+
+instance : Hashable Empty := ⟨nofun⟩
+
+def tasks : Incremental.Tasks Monad config
+  | 0 => pure 0
+  | 1 => pure 1
+  | n + 2 => do
+    let a ← Incremental.fetch (n + 1) (by omega)
+    let b ← Incremental.fetch n (by omega)
+    return a + b
+
+end Incremental.Test.Fibonacci
