Incremental/Test/Triangle.lean
@@ -1,0 +1,27 @@
+import Incremental.Basic
+
+namespace Incremental.Test.Triangle
+
+abbrev config : Incremental.BuildConfig where
+  I := Empty
+  V := nofun
+  Q := Nat
+  R _ := Nat
+  rel := (· < ·)
+  wf := Nat.lt_wfRel.wf
+
+instance : Incremental.Input config Unit where
+  get := nofun
+  set := nofun
+  get_set_self := nofun
+  get_set_other := nofun
+
+instance : Hashable Empty := ⟨nofun⟩
+
+def tasks : Incremental.Tasks Monad config
+  | 0 => pure 0
+  | n + 1 => do
+    let prev ← Incremental.fetch n (by omega)
+    return prev + (n + 1)
+
+end Incremental.Test.Triangle
